Softmax/LogSoftmax now have configurable nthr

src/klas/Klas.Softmax.fst
@@ -5,6 +5,12 @@ open Kuiper
 
 module K = Kuiper.Kernel.Softmax
 
-let softmax_f16 : K.softmax_ty f16 = K.softmax
-let softmax_f32 : K.softmax_ty f32 = K.softmax
-let softmax_f64 : K.softmax_ty f64 = K.softmax
+(* dynamic thread number *)
+let softmax_n_f16 : K.softmax_ty f16 = K.softmax
+let softmax_n_f32 : K.softmax_ty f32 = K.softmax
+let softmax_n_f64 : K.softmax_ty f64 = K.softmax
+
+(* full blocks. TODO: would it help to use smin lena 1024? *)
+let softmax_f16 lena = K.softmax #f16 1024sz #lena
+let softmax_f32 lena = K.softmax #f32 1024sz #lena
+let softmax_f64 lena = K.softmax #f64 1024sz #lena
