src/klas/Klas.LogSoftmax.fst
@@ -5,6 +5,12 @@ open Kuiper
 
 module K = Kuiper.Kernel.LogSoftmax
 
-let log_softmax_f16 : K.log_softmax_ty f16 = K.log_softmax
-let log_softmax_f32 : K.log_softmax_ty f32 = K.log_softmax
-let log_softmax_f64 : K.log_softmax_ty f64 = K.log_softmax
+(* dynamic thread number *)
+let log_softmax_n_f16 : K.log_softmax_ty f16 = K.log_softmax
+let log_softmax_n_f32 : K.log_softmax_ty f32 = K.log_softmax
+let log_softmax_n_f64 : K.log_softmax_ty f64 = K.log_softmax
+
+(* full blocks. TODO: would it help to use smin lena 1024? *)
+let log_softmax_f16 lena = K.log_softmax #f16 1024sz #lena
+let log_softmax_f32 lena = K.log_softmax #f32 1024sz #lena
+let log_softmax_f64 lena = K.log_softmax #f64 1024sz #lena
