src/klas/Klas.Softmax.fsti
@@ -4,6 +4,6 @@ module Klas.Softmax
 open Kuiper
 module K = Kuiper.Kernel.Softmax
 
-val softmax_f16 : K.softmax_ty f16
-val softmax_f32 : K.softmax_ty f32
-val softmax_f64 : K.softmax_ty f64
+val softmax_n_f16 : K.softmax_ty f16
+val softmax_n_f32 : K.softmax_ty f32
+val softmax_n_f64 : K.softmax_ty f64
